Rename stuff

src/Comparse.Parser.Typeclass.fst
@@ -4,23 +4,23 @@ open Comparse.Bytes.Typeclass
 open Comparse.Parser
 
 class parseable_serializeable (bytes:Type0) {|bytes_like bytes|} (a:Type) = {
-  [@@@FStar.Tactics.Typeclasses.no_method] base: parser_serializer_exact bytes a;
+  [@@@FStar.Tactics.Typeclasses.no_method] base: parser_serializer_whole bytes a;
 }
 
 val parse: #bytes:Type0 -> {|bytes_like bytes|} -> a:Type -> {|parseable_serializeable bytes a|} -> bytes -> option a
 let parse #bytes #bl a #ps buf =
-  ps.base.parse_exact buf
+  ps.base.parse buf
 
 val serialize: #bytes:Type0 -> {|bytes_like bytes|} -> a:Type -> {|parseable_serializeable bytes a|} -> a -> bytes
 let serialize #bytes #bl a #ps x =
-  ps.base.serialize_exact x
+  ps.base.serialize x
 
 val parse_serialize_inv_lemma: #bytes:Type0 -> {|bytes_like bytes|} -> a:Type -> {|parseable_serializeable bytes a|} -> x:a -> Lemma (
     // #bytes implicit argument needed to know to which bytes we are serializing to
     parse a (serialize #bytes a x) == Some x
   )
 let parse_serialize_inv_lemma #bytes #bl a #ps x =
-  ps.base.parse_serialize_inv_exact x
+  ps.base.parse_serialize_inv x
 
 val serialize_parse_inv_lemma: #bytes:Type0 -> {|bytes_like bytes|} -> a:Type -> {|parseable_serializeable bytes a|} -> buf:bytes -> Lemma (
     match parse a buf with
@@ -28,11 +28,11 @@ val serialize_parse_inv_lemma: #bytes:Type0 -> {|bytes_like bytes|} -> a:Type ->
     | None -> True
   )
 let serialize_parse_inv_lemma #bytes #bl a #ps buf =
-  ps.base.serialize_parse_inv_exact buf
+  ps.base.serialize_parse_inv buf
 
 val is_well_formed: #bytes:Type0 -> {|bytes_like bytes|} -> a:Type -> {|parseable_serializeable bytes a|} -> bytes_compatible_pre bytes -> a -> Type0
 let is_well_formed #bytes #bl a #ps pre x =
-  is_well_formed_exact ps.base pre x
+  is_well_formed_whole ps.base pre x
 
 val parse_wf_lemma: #bytes:Type0 -> {|bytes_like bytes|} -> a:Type -> {|parseable_serializeable bytes a|} -> pre:bytes_compatible_pre bytes -> buf:bytes -> Lemma
   (requires pre buf)
@@ -57,15 +57,15 @@ val wf_weaken_lemma: #bytes:Type0 -> {|bytes_like bytes|} -> a:Type -> {|parseab
 let wf_weaken_lemma #bytes #bl a #ps pre_strong pre_weak x =
   ()
 
-val mk_parseable_serializeable_from_exact:
+val mk_parseable_serializeable_from_whole:
   #bytes:Type0 -> {|bytes_like bytes|} -> #a:Type ->
-  pse_a:parser_serializer_exact bytes a -> parseable_serializeable bytes a
-let mk_parseable_serializeable_from_exact #bytes #bl #a pse_a = {
-  base = pse_a;
+  pswa:parser_serializer_whole bytes a -> parseable_serializeable bytes a
+let mk_parseable_serializeable_from_whole #bytes #bl #a ps_a = {
+  base = ps_a;
 }
 
 val mk_parseable_serializeable:
   #bytes:Type0 -> {|bytes_like bytes|} -> #a:Type ->
   ps_a:parser_serializer bytes a -> parseable_serializeable bytes a
 let mk_parseable_serializeable #bytes #bl #a ps_a =
-  mk_parseable_serializeable_from_exact (ps_to_pse ps_a)
+  mk_parseable_serializeable_from_whole (ps_prefix_to_ps_whole ps_a)
